\section{Problems}
\begin{homeworkProblem}
    求证
    \[
        \oint_{\vert z \vert = r > 1} \frac{1}{1+z^n}{\mathrm{d}z}
        = \oint_{\vert z \vert = r > 1} \frac{z^{2n}}{1+z^n}{\mathrm{d}z}
        = \left\{ \begin{array}{ll}
        2\pi i & n = 1 \\
        0 & n \ge 2 \end{array} \right
    \]
\textbf{\large Solution 1}
    \[
        \begin{equation*}
            \begin{split}
                \oint_{\vert z \vert = r > 1} \frac{1}{1+z^n}{\mathrm{d}z}
                & = 2\pi i \sum_{k=1}^{n}\Res [\frac{1}{1+z^n}, z_k] \\
                & = 2\pi i \sum_{k=1}^{n}\frac{1}{nz_{k}^{n-1}} \\
                & = \frac{2\pi i}{n}\sum_{k=1}^{n}\frac{1}{z_{k}^{n-1}}
            \end{split}
        \end{equation*}
    \]
    注意到 \[ z_k^n = 1 \] 则 \[ -z_k = \frac{1}{z_k^{n-1}} \]
    因此
    \[
    \begin{split}
        &\oint_{\vert z \vert = r > 1} \frac{1}{1+z^n}{\mathrm{d}z}\\
        =& \frac{2\pi i}{n}\sum_{k=1}^{n}\frac{1}{z_{k}^{n-1}}\\
        =& -\frac{2\pi i}{n}\sum_{k=1}^{n}z_k
    \end{split}
    \]
    若 $n = 1$，即 \[1 + z^n = 1 + z= 0\] 解得 \[z=-1\] 因此
    \[\oint_{\vert z \vert = r > 1} \frac{1}{1+z^n}{\mathrm{d}z} = 2\pi i\]
    否则 \[\sum_{k=1}^n z_k = 0\]
    即 \[\oint_{\vert z \vert = r > 1} \frac{1}{1+z^n}{\mathrm{d}z} = 0\]
    又
    \[\begin{split}
    \oint_{\vert z \vert = r > 1}\frac{z^{2n}}{1+z^n}\mathrm{d}z
    & = \oint_{\vert z \vert = r > 1}\frac{(z^{2n} - 1) + 1}{1+z^n} \mathrm{d}z\\
    & = \oint_{\vert z \vert = r > 1}\frac{(z^{n} - 1)(z^{n} + 1)}{1+z^n}\mathrm{d}z + \oint_{\vert z \vert = r > 1}\frac{1}{1+z^n}\mathrm{d}z \\
    & = \oint_{\vert z \vert = r > 1}(z^{n} - 1)\mathrm{d}z + \oint_{\vert z \vert = r > 1}\frac{1}{1+z^n}\mathrm{d}z
    \end{split}\]
    由Cauchy-Goursat定理 \[\oint_{\vert z \vert = r > 1}(z^{n} - 1)\mathrm{d}z  = 0\]
    所以 \[\oint_{\vert z \vert = r > 1} \frac{1}{1+z^n}{\mathrm{d}z}
    = \oint_{\vert z \vert = r > 1} \frac{z^{2n}}{1+z^n}{\mathrm{d}z}\]
    综上，
    \[
    \oint_{\vert z \vert = r > 1} \frac{1}{1+z^n}{\mathrm{d}z}
    = \oint_{\vert z \vert = r > 1} \frac{z^{2n}}{1+z^n}{\mathrm{d}z}
    = \left\{ \begin{array}{ll}
    2\pi i & n = 1 \\
    0 & n \ge 2 \end{array} \right
    \]
\textbf{\large Solution 2}\newline
令$z=re^{i\theta}\quad 0\le\theta<\2\pi,t=\frac{1}{z}$，则
\begin{gather*}
    |t| = \frac{1}{r} < 1\\
    t=\frac{1}{r}e^{-i\theta}\\
    \mathrm{d}z = \mathrm{d}(\frac{1}{t})=-\frac{1}{t^2}\mathrm{d}t\qquad0\le\theta<\2\pi\quad\textrm{积分方向为顺时针}
\end{gather*}
此时原积分
\[
\begin{split}
    \oint_{\vert z \vert = r > 1} \frac{1}{1+z^n}{\mathrm{d}z}
    &= -\oint_{|t|=\frac{1}{r}<1}\frac{1}{1+\frac{1}{t^2}}(-\frac{1}{t^2})\mathrm{d}t\\
    &= \oint_{|t|=\frac{1}{r}<1}\frac{t^{n-2}}{1+t^n}\mathrm{d}t
\end{split}
\]
只有一个奇点$t=0$。因此
\[
\begin{split}
    I_n
    &= \oint_{|t|=\frac{1}{r}<1}\frac{t^{n-2}}{1+t^n}\mathrm{d}t\\
    &=\left\bigg\{\begin{array}{ll}0& n\geq2\qquad\textrm{(Cauchy-Goursat 定理)} \\
    \oint_{|t|=\frac{1}{r}<1}\frac{1}{t(t+1)}\mathrm{d}t=2\pi i & n=1
    \end{array}\right
\end{split}
\]
\end{homeworkProblem}

\begin{homeworkProblem}
    求积分
    \[
    \oint_{|z| = r > 0}\frac{1-\cos4z^3}{z^n}\mathrm{d}z \qquad n\in\mathbb{Z}
    \]

\solution
当$n\leq 0$时
\[
\oint_{|z| = r > 0}\frac{1-\cos4z^3}{z^n}\mathrm{d}z = 0
\]
当$n > 0$时
\[\begin{split}
\frac{1-\cos4z^3}{z^n}
&=z^{-n}(1-\sum_{k=0}^n(-1)^k\frac{(4z^3)^{2k}}{(2k)!})\\
&=z^{-n}(1-\sum_{k=0}^n(-1)^k\frac{4^{2k}z^{6k}}{(2k)!})\\
&=z^{-n}\sum_{k=1}^n(-1)^{k-1}\frac{4^{2k}z^{6k}}{(2k)!}\\
\end{split}\]
$\frac{1-\cos4z^3}{z^n}$在奇点$z=0$的Laurent级数$\sum_{n=-\infty}^{+\infty}C_nz^n$中，$C_{-1}$对应上式中
\[
6k-n=-1
\]
此时
\[\begin{split}
C_{-1}&=(-1)^{k-1}\frac{4^{2k}}{(2k)!}\qquad{k=\frac{n-1}{6}}\\
&=(-1)^{\frac{n-7}{6}}\frac{4^{\frac{n-1}{3}}}{(\frac{n-1}{3})!}
\end{split}\]
所以$n > 0$时
\[\begin{split}
\oint_{|z| = r > 0}\frac{1-\cos4z^3}{z^n}\mathrm{d}z
&=2\pi i\Res[\frac{1-\cos4z^3}{z^n}, 0]\\
&=2\pi i C_{-1}\\
&=2\pi i(-1)^{\frac{n-7}{6}}\frac{4^{\frac{n-1}{3}}}{(\frac{n-1}{3})!}
\end{split}\]
综上，
\[\begin{split}
\oint_{|z| = r > 0}\frac{1-\cos4z^3}{z^n}\mathrm{d}z
= \left\{\begin{array}{ll}
2\pi i(-1)^{\frac{n-7}{6}}\cfrac{4^{\frac{n-1}{3}}}{(\frac{n-1}{3})!} & n=6k+1, k\in\mathbb{N} \\
0 & n\neq 6k+1, k\in\mathbb{N}\end{array}\right
\end{split}\]
\end{homeworkProblem}

\begin{homeworkProblem}
    求积分
    \[
    \oint_{|z| = r > 1}\frac{z^3 e^\frac{1}{z}}{1+z}\mathrm{d}z
    \]
\solution
令$t=\frac{1}{z}$,则
\begin{gather*}
    |t| = \frac{1}{r} < 1\\
    t=\frac{1}{r}e^{-i\theta}\\
    \mathrm{d}z = \mathrm{d}(\frac{1}{t})=-\frac{1}{t^2}\mathrm{d}t\qquad0\le\theta<\2\pi\quad\textrm{积分方向为顺时针}
\end{gather*}
原积分
\[\begin{split}
\oint_{|z| = r > 1}\frac{z^3 e^\frac{1}{z}}{1+z}\mathrm{d}z
&= -\oint_{|t| = \frac{1}{r} < 1}\frac{e^t}{t^2(t+1)}(-\frac{1}{t^2})\mathrm{d}t \\
&= \oint_{|t| = \frac{1}{r} < 1}\frac{e^t}{t^4(t+1)}\mathrm{d}t \\
&= 2\pi i\Res[\frac{e^t}{t^4(t+1)}, 0]
\end{split}\]
又
\[\begin{split}
\frac{e^t}{t^4(t+1)} &= t^{-4}(1+t+\frac{t^2}{2!}+\frac{t^3}{3!}+\dots)(1-t+t^2-t^3+\dots)
\end{split}\]
其中，$t^{-1}$的系数为
\[-1+1-\frac{1}{2!}+\frac{1}{3!} = -\frac{1}{3}\]
因此
\[\oint_{|z| = r > 1}\frac{z^3 e^\frac{1}{z}}{1+z}\mathrm{d}z
=2\pi i\Res[\frac{e^t}{t^4(t+1)}, 0]
=2\pi i (-\frac{1}{3})
=-\frac{2}{3}\pi i\]
\end{homeworkProblem}
\begin{homeworkProblem}
    求积分
    \[
    \int_0^{2\pi}\frac{\mathrm{d}\theta}{a+b\cos\theta} \qquad a>|b|\quad a,b\in\mathbb{R}
    \]
\solution
令$z=e^{i\theta}, \theta\in[0, 2\pi)$，注意到:
\begin{gather*}
\cos\theta = \frac{e^{i\theta}+e^{-i\theta}}{2}=\frac{z+\frac{1}{z}}{2}=\frac{z^2+1}{2z}\\
\mathrm{d}\theta = \frac{\mathrm{d}z}{ie^{i\theta}}=\frac{\mathrm{d}z}{iz}\\
\end{gather*}
则原积分
\[\begin{split}
\int_0^{2\pi}\frac{\mathrm{d}\theta}{a+b\cos\theta}
&= \oint_{|z|=1}\cfrac{\frac{\mathrm{d}z}{iz}}{a+b(\frac{z^2+1}{2z})}\\
&=\frac{2}{i}\oint_{|z|=1}\frac{\mathrm{d}z}{bz^2+2az+b}
\end{split}\]
当$b=0$时，原积分
\[\int_0^{2\pi}\frac{\mathrm{d}\theta}{a+b\cos\theta}
=\int_0^{2\pi}\frac{\mathrm{d}\theta}{a}
=\frac{2\pi}{a}\]
当$b\neq0$时，原积分
\[\begin{split}\int_0^{2\pi}\frac{\mathrm{d}\theta}{a+b\cos\theta}
&=\frac{2}{i}\oint_{|z|=1}\frac{\mathrm{d}z}{bz^2+2az+b}\\
&=\frac{2}{ib}\oint_{|z|=1}\frac{\mathrm{d}z}{z^2+\frac{2a}{b}z+1}
\end{split}\]
对方程\[z^2+\frac{2a}{b}z+1=0\]其两根\[z_1z_2=1\]且
\[z_{1,2}=-\frac{a}{b}\pm\frac{\sqrt{a^2-b^2}}{b}\]
可设$b>0$，则
\[z_2 =-\frac{a}{b}\-\frac{\sqrt{a^2-b^2}}{b}<-\frac{a}{b}<-1\]
即只有一个奇点$z_1$。所以原积分
\[\begin{split}
\int_0^{2\pi}\frac{\mathrm{d}\theta}{a+b\cos\theta}
&=\frac{2}{ib}\oint_{|z|=1}\frac{\mathrm{d}z}{z^2+\frac{2a}{b}z+1}\\
&=\frac{2}{ib}2\pi i\frac{1}{2z_1+\frac{2a}{b}}\\
&=\frac{2\pi}{\sqrt{a^2-b^2}}
\end{split}\]
\end{homeworkProblem}
\begin{homeworkProblem}
    求积分
    \[
    \int_0^{2\pi}\frac{\mathrm{d}\theta}{a+b\sin\theta} \qquad a>|b|\quad a,b\in\mathbb{R}
    \]
\solution
\begin{theorem*}
    若$f(x)$在$[-1,1]$上可积，则$\int_0^{2\pi}f(\cos x)\dtheta=\int_0^{2\pi}f(\sin x)\dtheta$
\end{theorem*}
所以
\[\int_0^{2\pi}\frac{\mathrm{d}\theta}{a+b\sin\theta}=\int_0^{2\pi}\frac{\mathrm{d}\theta}{a+b\cos\theta}=\frac{2\pi}{\sqrt{a^2-b^2}}\]
\end{homeworkProblem}
\begin{homeworkProblem}
    求积分
    \[
    I_p = \int_0^{2\pi}\frac{\mathrm{d}\theta}{1-2p\cos\theta+p^2}\qquad p\in(-1,1)
    \]
\solution
令
\begin{gather*}
a=1+p^2\\
b=-2p
\end{gather*}
则\[a>b\quad a,b\in(-1,1)\]
因此
\[\begin{split}
I_p
&= \int_0^{2\pi}\frac{\mathrm{d}\theta}{1-2p\cos\theta+p^2}\\
&= \int_0^{2\pi}\frac{\mathrm{d}\theta}{a+b\cos\theta}\\
&=\frac{2\pi}{\sqrt{a^2-b^2}} \\
&=\frac{2\pi}{1-p^2}
\end{split} \]
\end{homeworkProblem}
\begin{homeworkProblem}
    求积分
    \[
    I_{A,B} = \int_0^{2\pi}\frac{\dtheta}{A^2\cos^2\theta + B^2\sin^2\theta}
    \qquad A,B\in\mathbb{R}\quadAB>0
    \]
\solution
令
\begin{gather*}
\cos^2\theta = \frac{\cos2\theta+1}{2}\\
\sin^2\theta = \frac{1-\cos2\theta}{2}
\end{gather*}
则
\[\begin{split}
I_{A,B} &= \int_0^{2\pi}\frac{\dtheta}{A^2\cos^2\theta + B^2\sin^2\theta}\\
&= \int_0^{2\pi}\cfrac{\dtheta}{A^2\cfrac{\cos2\theta+1}{2} + B^2\cfrac{1-\cos2\theta}{2}} \\
&= \int_0^{4\pi}\frac{\mathrm{d}t}{(A^2+B^2)+(A^2-B^2)\cos t}\\
&= 2\int_0^{2\pi}\frac{\mathrm{d}t}{(A^2+B^2)+(A^2-B^2)\cos t}\\
&=2\frac{2\pi}{\sqrt{(A^2+B^2)^2-(A^2-B^2)^2}}\\
&=\frac{2\pi}{AB}
\end{split}\]
\end{homeworkProblem}

\begin{homeworkProblem}
    求积分
    \[I_n=\int_0^{+\infty}\frac{1}{(x^2+a^2)(x^2+b^2)}\dx\]
\solution
$\frac{1}{(x^2+a^2)(x^2+b^2)}$是偶函数，因此
\[\begin{split}
I_n&=\int_0^{+\infty}\frac{1}{(x^2+a^2)(x^2+b^2)}\dx\\
&=\frac{1}{2}\int_{-\infty}^{+\infty}\frac{1}{(x^2+a^2)(x^2+b^2)}\\
&=\frac{1}{2}\lim{R \rightarrow +\infty}\int_{-R}^{+R}\frac{1}{(x^2+a^2)(x^2+b^2)}
\end{split}\]
而
\[\begin{split}
&\lim_{R \rightarrow +\infty}\int_{-R}^{+R}\frac{1}{(x^2+a^2)(x^2+b^2)}
+ \int_{|z|=R, Im[z]>0}\frac{1}{(z^2+a^2)(z^2+b^2)}\mathrm{d}z\\
=& 2\pi i(\Res[\frac{1}{(x^2+a^2)(x^2+b^2)}, i|a|] + \Res[\frac{1}{(x^2+a^2)(x^2+b^2)}, i|b|])\\
=& 2\pi i(\frac{1}{4(i|a|)^3+2i|a|(a^2+b^2)+ab}+\frac{1}{4(i|b|)^3+2i|b|(a^2+b^2)+ab})
\end{split}\]
\begin{theorem*}
    若$P_n(z),Q_m(z)$是多项式，且$degP_n = n \leq degQ_m-2=m-2$，$Q_m(z)$在实轴$z=x$上没有零点，即$Q_m(x)\neq0,\forall x\in\mathbb{R}$，则$\lim_{R\rightarrow +\infty}\int_{|z|=R, Im[z]>0}\frac{P_n(z)}{Q_m(z)}\mathrm{d}z=0$
\end{theorem*}
所以
\[\begin{split}
I_n &= \frac{1}{2}2\pi i(\Res[\frac{1}{(x^2+a^2)(x^2+b^2)}, i|a|] + \Res[\frac{1}{(x^2+a^2)(x^2+b^2)}, i|b|])\\
&=\pi i(\frac{1}{4(i|a|)^3+2i|a|(a^2+b^2)+ab}+\frac{1}{4(i|b|)^3+2i|b|(a^2+b^2)+ab})
\end{split}\]
\end{homeworkProblem}

\begin{homeworkProblem}
    求积分
    \[
    I_{n} = \int_0^{+\infty}\frac{\dx}{1+x^{2n}}\qquad n\in\mathbb{N}
    \]
\end{homeworkProblem}
\begin{homeworkProblem}
    求积分
    \[
    I_{n,r} = \int_0^{+\infty}\frac{\dx}{r^{2n}+x^{2n}}\qquad n\in\mathbb{N}
    \]
\end{homeworkProblem}
\begin{homeworkProblem}
    求积分
    \[
    J_n = \int_0^{+\infty}\frac{\dx}{(1+x^2)^n} \qquad n\in\mathbb{N}
    \]
\end{homeworkProblem}
\begin{homeworkProblem}
    求积分
    \[
    J_n = \int_0^{+\infty}\frac{\dx}{(r^2+x^2)^n} \qquad n\in\mathbb{N}
    \]
\end{homeworkProblem}
\begin{homeworkProblem}
    求积分
    \[
    I_{a,b,k} = \int_0^{+\infty}\frac{x\sin kx}{(x^2+a^2)(x^2+b^2)}\dx
    \]
\end{homeworkProblem}
\begin{homeworkProblem}
    求积分
    \[
    I_{a,b,k} = \int_0^{+\infty}\frac{x^2\cos kx}{(x^2+a^2)(x^2+b^2)}\dx
    \]
\end{homeworkProblem}
